mostly-working testing harness and interpeter. parsing bytes into instructions seems to cause problems with the code generator due to the use of free_constructors. otherwise it seems to work. tests aren't yet passing.

EvmTests/translate_all_tests.rb
@@ -1,0 +1,24 @@
+#!/usr/bin/env ruby
+# Automation for generating all tests present in the provided Tests directory
+
+translate_script = "./translate_test.rb"
+
+if ARGV.length < 1 then
+  abort("Provide a directory to compile tests from")
+end
+
+target = ARGV[0]
+
+files = Dir.children "#{target}"
+
+puts "Translating tests from ./#{target}"
+
+for file_rel in files
+  if (/\.json$/ =~ file_rel)
+  then
+    file = "./" + target + "/" + file_rel
+    puts "Translating #{file}"
+    system("ruby", translate_script, file)
+  end
+end
+
