EvmTests/translate_test.rb
@@ -1,4 +1,7 @@
+#!/usr/bin/env ruby
 require 'json'
+
+# TODO: make this more robust w/r/t directory structure
 
 lllc_file = '/mnt/c/Users/yorix/winhome/Code/solidity/build/lllc/lllc'
 
@@ -10,6 +13,8 @@ name_j = ARGV[0]
 name_t = name_j.gsub ".json", ".thy"
 name_l = name_j.gsub ".json", ".lll"
 name_b = name_j.gsub ".json", ".out"
+name_stem1 = name_j.gsub ".json", ""
+name_stem = name_stem1.gsub(/^.*\//, "") 
 
 f_json = File.open(name_j, "r")
 obj = JSON.load f_json
@@ -22,53 +27,118 @@ File.open(name_l, "w") { |f|
   f.write lll_code
 }
 
+def drop0x(str)
+  if(str.nil?)
+    ""
+  else
+    if(str[0..1] == "0x")
+      if(str == "0x")
+      then
+        "0" # sometimes zero is annotated this way in the test cases...
+      else
+        str[2..]
+      end
+    else
+      str
+    end
+  end
+end
+
+def select_parser(str)
+  if(str[0..1] == "0x")
+    "parse_hex_str_eint"
+  else
+    "parse_dec_str_eint"
+  end
+end
+
+def parse_storage(obj, keys)
+  if keys == []
+  then
+    ""
+  else
+    out = "(#{select_parser (keys[0])} ''#{drop0x keys[0]}'', #{select_parser (obj[keys[0]])} ''#{drop0x obj[keys[0]]}'')"
+    if keys.length > 1 then
+      out + " , " + parse_storage(obj, keys[1..])
+    else
+      out
+    end
+  end
+end
+
 system(lllc_file, name_l, "-x", :out => [name_b, "w"])
 
 f_b = File.open(name_b, "r")
 
-bin_code = f_b.read
+bin_code = f_b.read.gsub("\n", "")
+
+puts bin_code
 
 
-f_thy = File.open(name_t, "w")
-
-=begin
-
-env:
-- currentCoinbase, 
-- currentDifficulty
-- currentGasLimit
-- currentNumber
-- currentTimestamp
-- previousHash
-
-exec:
--address, caller, data, gas, gasPrice, origin, value
-
-pre:
-- account (the hash)
-  - balance
-  - code
-  - nonce
-  - storage
-
-expect: (this is the key part)
-- account (the hash)
-  - storage
-    - mapping from keys to values
-      (special case "0x => 0")
-
-storage seems to be the only expect...
-
-=end
+# TODO: probably need to explicitly call toString in a bunch of places.
 
 
-# File.open(name_j, "r") do |f_json|
-#   obj = JSON.load f_json
+template =
+%Q`
+theory #{name_stem}
+imports "../../../Utils/Hex" "../../../EVM/EvmInterpreter" "../../test_utils"
+begin
+definition prog :: "8 word list" where
+"prog = hex_splits ''#{bin_code}''"
 
-#   # puts obj
-  
-#   File.open(name_t, "w") do |f_thy|
-    
-#   end
-# end
+definition input_storage where
+"input_storage = create_storage [#{parse_storage obj[prog]["pre"][contract]["storage"], obj[prog]["pre"][contract]["storage"].keys}]"
 
+definition output_storage where
+"output_storage = [#{parse_storage obj[prog]["expect"][contract]["storage"], obj[prog]["expect"][contract]["storage"].keys}]"
+
+definition  init_Estate :: "estate_ll" where
+"init_Estate =
+(dummy_estate_ll
+(| el_e :=
+  (dummy_estate
+    (| e_coinbase := #{select_parser (obj[prog]["env"]["currentCoinbase"])} ''#{drop0x obj[prog]["env"]["currentCoinbase"]}''
+     , e_difficulty := #{select_parser(obj[prog]["env"]["currentDifficulty"])} ''#{drop0x obj[prog]["env"]["currentDifficulty"]}''
+     , e_gaslimit := #{select_parser(obj[prog]["env"]["currentGasLimit"])} ''#{drop0x obj[prog]["env"]["currentGasLimit"]}''
+     , e_blocknumber := #{select_parser(obj[prog]["env"]["currentNumber"])} ''#{drop0x obj[prog]["env"]["currentNumber"]}''
+     , e_timestamp := #{select_parser(obj[prog]["env"]["currentTimestamp"])} ''#{drop0x obj[prog]["env"]["currentTimestamp"]}''
+     , e_blockhash := parse_hex_str_eint ''#{drop0x obj[prog]["env"]["previousHash"]}''
+
+     , e_address := parse_hex_str_eint ''#{drop0x obj[prog]["exec"]["address"]}''
+     , e_caller := parse_hex_str_eint ''#{drop0x obj[prog]["exec"]["caller"]}''
+     , e_calldata := hex_splits ''#{drop0x obj[prog]["exec"]["data"]}''
+     , e_gas := #{select_parser (obj[prog]["exec"]["gas"])} ''#{drop0x obj[prog]["exec"]["gas"]}''
+     , e_gasprice := #{select_parser obj[prog]["exec"]["gasPrice"]} ''#{drop0x obj[prog]["exec"]["gasPrice"]}''
+     , e_origin := parse_hex_str_eint ''#{drop0x obj[prog]["exec"]["origin"]}''
+     , e_callvalue := #{select_parser (obj[prog]["exec"]["gas"])} ''#{drop0x obj[prog]["exec"]["value"]}''
+     
+     , e_selfbalance := #{select_parser (obj[prog]["pre"][contract]["balance"])} ''#{drop0x obj[prog]["pre"][contract]["balance"]}''
+     , e_codedata := hex_splits ''#{bin_code}''
+     , e_nonce := #{select_parser (obj[prog]["pre"][contract]["nonce"])} ''#{drop0x obj[prog]["pre"][contract]["nonce"]}''
+     , e_storage := input_storage
+    |))
+|))"
+
+definition final_Estate :: "estate_ll option" where
+"final_Estate = evm_exec init_Estate"
+
+definition final_check :: "bool" where
+"final_check =
+  (case final_Estate of
+    None => False
+    | Some e => check_storage e output_storage)"
+
+(* value "final_estate" *)
+
+(*
+ * Iff this returns true, the test has succeeded.
+ *)
+value "final_check"
+end
+`
+
+puts "writing output..."
+
+f_thy = File.open(name_t, "w") { |f|
+  f.write template
+}
