EVM/EvmInterpreter.thy
@@ -1,11 +1,12 @@
-theory EvmInterpreter imports EvmBytecode MiniEvm "HOL-Library.Adhoc_Overloading"
+theory EvmInterpreter imports EvmBytecode MiniEvm "HOL-Library.Adhoc_Overloading" "../Utils/Hex"
 begin
 
-(*
-definition parse_byte_inst' :: "8 word \<Rightarrow> nat" where
-"parse_byte_inst' w = unat w"
+(* parsing hex inputs 
+ * because of the free constructors (I think) we can't define
+   this directly, which would be the natural thing to do.
 *)
 
+(*
 lift_definition parse_byte_inst :: "8 word \<Rightarrow> inst"
 is unat
 proof-
@@ -20,6 +21,19 @@ proof-
       by simp
   qed
 qed
+
+value "parse_byte_inst 0"
+*)
+(*
+ * Begin the actual interpreter
+ *)
+
+definition parse_hex_str_eint :: "char list \<Rightarrow> eint" where
+"parse_hex_str_eint l = word_rcat (hex_splits l)"
+
+definition parse_dec_str_eint :: "char list \<Rightarrow> eint" where
+"parse_dec_str_eint l = word_of_int (decread l)"
+
 
 (* add stack, pc to estate *)
 record estate_ll =
@@ -322,8 +336,6 @@ fun swap' :: "nat \<Rightarrow> 'a list \<Rightarrow> 'a list option" where
         | sth#stt \<Rightarrow>
            Some ((stt ! n) # take n stt @ (sth # (drop (n+1) stt)))))"
 
-value "swap' 1 [(2 :: nat), 3, 4, 5]"
-
 (* el_swap 0 <==> SWAP1 *)
 fun el_swap :: "nat \<Rightarrow> el_step" where
 "el_swap n el =
@@ -354,20 +366,186 @@ fun el_push :: "nat \<Rightarrow> el_step" where
            (el \<lparr> el_pc := pc + n' + 2
                , el_stack := word_rcat bytes # el_stack el \<rparr>))))))))"
 
-(* TODO *)
 fun el_jump :: "el_step" where
-"el_jump x = x"
+"el_jump el = 
+  (case el_stack el of
+   [] \<Rightarrow> crash el
+   | h#t \<Rightarrow>
+     (el \<lparr> el_pc := h
+         , el_stack := t \<rparr>))
+"
 
 fun el_jumpi :: "el_step" where
-"el_jumpi x = x"
+"el_jumpi el = 
+  (case el_stack el of
+    dst#cond#t \<Rightarrow>
+      (if cond = 0
+       then
+        (if el_pc el = max_ueint then crash el
+         else (el \<lparr> el_pc := el_pc el + 1
+                  , el_stack := t \<rparr>))
+        else (el \<lparr> el_pc := dst
+                 , el_stack := t \<rparr>))
+    | _ \<Rightarrow> crash el)"
 
 fun el_jumpdest :: "el_step" where
-"el_jumpdest x = x"
+"el_jumpdest el = 
+  (if el_pc el = max_ueint then crash el
+   else (el \<lparr> el_pc := el_pc el + 1 \<rparr>))"
 
 fun el_getpc :: "el_step" where
-"el_getpc x = x"
+"el_getpc el = 
+  (if el_pc el = max_ueint then crash el
+  else (el \<lparr> el_stack := (el_pc el) # el_stack el
+           , el_pc := el_pc el + 1 \<rparr>))"
 
 fun el_getgas :: "el_step" where
-"el_getgas x = x"
+"el_getgas el = 
+  (if el_pc el = max_ueint then crash el
+   else (el \<lparr> el_stack := e_gas (el_e el) # el_stack el
+            , el_pc := el_pc el + 1 \<rparr>))"
+
+fun get_inst :: "estate_ll \<Rightarrow> inst" where
+"get_inst el =
+  (if unat (el_pc el) < length (e_codedata (el_e el)) then eSTOP
+   else parse_byte_inst (e_codedata (el_e el) ! (unat (el_pc el))))"
+
+
+
+(*
+ * Semantics of a single instruction execution
+ *)
+fun el_step :: "inst \<Rightarrow> el_step" where
+"el_step eSTOP = mkStep ei_stop"
+| "el_step eADD = mkStep ei_add"
+| "el_step eMUL = mkStep ei_mul"
+| "el_step eSUB = mkStep ei_sub"
+| "el_step eDIV = mkStep ei_div"
+| "el_step eSDIV = mkStep ei_sdiv"
+| "el_step eMOD = mkStep ei_mod"
+| "el_step eSMOD = mkStep ei_smod"
+| "el_step eADDMOD = mkStep ei_addmod"
+| "el_step eMULMOD = mkStep ei_mulmod"
+| "el_step eEXP = mkStep ei_exp"
+| "el_step eSIGNEXTEND = mkStep ei_signextend"
+| "el_step eLT = mkStep ei_lt"
+| "el_step eGT = mkStep ei_gt"
+| "el_step eSLT = mkStep ei_slt"
+| "el_step eSGT = mkStep ei_sgt"
+| "el_step eEQ = mkStep ei_eq"
+| "el_step eISZERO = mkStep ei_iszero"
+| "el_step eAND = mkStep ei_and"
+| "el_step eOR = mkStep ei_or"
+| "el_step eXOR = mkStep ei_xor"
+| "el_step eNOT = mkStep ei_not"
+| "el_step eBYTE = mkStep ei_byte"
+| "el_step eSHL = mkStep ei_shl"
+| "el_step eSHR = mkStep ei_shr"
+| "el_step eSAR = mkStep ei_sar"
+| "el_step eKECCAK256 = mkStep ei_keccak256"
+| "el_step eADDRESS = mkStep ei_address"
+| "el_step eBALANCE = mkStep ei_balance"
+| "el_step eORIGIN = mkStep ei_origin"
+| "el_step eCALLER = mkStep ei_caller"
+| "el_step eCALLVALUE = mkStep ei_callvalue"
+| "el_step eCALLDATALOAD = mkStep ei_calldataload"
+| "el_step eCALLDATASIZE = mkStep ei_calldatasize"
+| "el_step eCALLDATACOPY = mkStep ei_calldatacopy"
+| "el_step eCODESIZE = mkStep ei_codesize"
+| "el_step eCODECOPY = mkStep ei_codecopy"
+| "el_step eGASPRICE = mkStep ei_gasprice"
+| "el_step eEXTCODESIZE = mkStep ei_extcodesize"
+| "el_step eEXTCODECOPY = mkStep ei_extcodecopy"
+| "el_step eRETURNDATASIZE = mkStep ei_returndatasize"
+| "el_step eRETURNDATACOPY = mkStep ei_returndatacopy"
+| "el_step eEXTCODEHASH = mkStep ei_extcodehash"
+| "el_step eBLOCKHASH = mkStep ei_blockhash"
+| "el_step eCOINBASE = mkStep ei_coinbase"
+| "el_step eTIMESTAMP = mkStep ei_timestamp"
+| "el_step eNUMBER = mkStep ei_number"
+| "el_step eDIFFICULTY = mkStep ei_difficulty"
+| "el_step eCHAINID = mkStep ei_chainid"
+| "el_step eSELFBALANCE = mkStep ei_selfbalance"
+| "el_step ePOP = mkStep ei_pop"
+| "el_step eMLOAD = mkStep ei_mload"
+| "el_step eMSTORE = mkStep ei_mstore"
+| "el_step eMSTORE8 = mkStep ei_mstore8"
+| "el_step eSLOAD = mkStep ei_sload"
+| "el_step eSSTORE = mkStep ei_sstore"
+| "el_step eJUMP = el_jump"
+| "el_step eJUMPI = el_jumpi"
+| "el_step ePC = el_getpc"
+| "el_step eMSIZE = mkStep ei_msize"
+| "el_step eGAS = mkStep ei_gas"
+| "el_step eJUMPDEST = mkStep ei_jumpdest"
+| "el_step eLOG0 = mkStep ei_log0"
+| "el_step eLOG1 = mkStep ei_log1"
+| "el_step eLOG2 = mkStep ei_log2"
+| "el_step eLOG3 = mkStep ei_log3"
+| "el_step eLOG4 = mkStep ei_log4"
+| "el_step eCREATE = mkStep ei_create"
+| "el_step eCALL = mkStep ei_call"
+| "el_step eCALLCODE = mkStep ei_callcode"
+| "el_step eRETURN = mkStep ei_return"
+| "el_step eDELEGATECALL = mkStep ei_delegatecall"
+| "el_step eCREATE2 = mkStep ei_create2"
+| "el_step eSTATICCALL = mkStep ei_staticcall"
+| "el_step eREVERT = mkStep ei_revert"
+| "el_step eINVALID = mkStep ei_invalid"
+| "el_step eSELFDESTRUCT = mkStep ei_selfdestruct"
+| "el_step _ = mkStep ei_invalid"
+
+
+(* execution *)
+fun evm_exec' :: "estate_ll \<Rightarrow> nat \<Rightarrow> estate_ll option" where
+"evm_exec' el 0 = None"
+| "evm_exec' el (Suc n) =
+   (if is_Executing (e_flag (el_e el))
+    then
+      (if el_crash el then Some el
+       else
+        (let next_inst = get_inst el in
+        (let next_state = el_step next_inst el in
+         evm_exec' next_state n)))
+    else Some el)"
+
+definition evm_exec :: "estate_ll \<Rightarrow> estate_ll option" where
+"evm_exec el = evm_exec' el 10000"
+
+definition evm_exec_check :: "estate_ll \<Rightarrow> (estate_ll \<Rightarrow> bool) \<Rightarrow> bool" where
+"evm_exec_check el P =
+ (case evm_exec el of
+  None \<Rightarrow> False
+  | Some final \<Rightarrow> P final)"
+
+(*
+ * storage
+*)
+type_synonym storage_spec = "(eint * eint) list"
+
+fun setup_storage :: "storage_spec \<Rightarrow> (eint \<Rightarrow> eint)" where
+"setup_storage [] i = 0"
+| "setup_storage ((k, v)#t) i =
+   (if i = k then v
+    else setup_storage t i)"
+
+(*
+check final storage 
+   NB: this does not check that unspecified
+   storage locations must be empty (0)
+*)
+fun check_storage :: "estate_ll \<Rightarrow> storage_spec \<Rightarrow> bool" where
+"check_storage el [] = True"
+| "check_storage el ((k, v)#t) =
+   ((e_storage (el_e el) k = v) \<and> check_storage el t)"
+
+
+(* starting state *)
+definition dummy_estate_ll :: "estate_ll" where
+"dummy_estate_ll =
+  \<lparr> el_e = dummy_estate
+  , el_stack = []
+  , el_pc = 0
+  , el_crash = False \<rparr>"
 
 end
