EvmTests/test_utils.thy
@@ -1,0 +1,21 @@
+theory test_utils
+imports Main "../Utils/Hex" "../EVM/MiniEvm"
+begin
+
+(* read in data blocks from hex *)
+
+(* read in code from hex *)
+
+
+fun check_expect_storage :: "((eint * eint) list) \<Rightarrow> estate \<Rightarrow> bool" where
+"check_expect_storage [] st = True"
+| "check_expect_storage ((idx,val)#t) st =
+   ((e_storage st idx = val) \<and>
+    check_expect_storage t st)"
+
+fun create_storage :: "((eint * eint) list) \<Rightarrow> eint \<Rightarrow> eint" where
+"create_storage [] = (\<lambda> _ . 0)"
+| "create_storage ((k,v)#t) =
+  (\<lambda> k' . (if k = k' then v else create_storage t k'))"
+
+end
