EvmTests/README.md
@@ -1,2 +1,14 @@
 Based on test suite from
 https://github.com/ethereum/tests/blob/develop/src/VMTestsFiller
+
+Copy from here into Tests.
+
+Then run e.g.
+
+"ruby ./translate_all_tests.rb ./Tests/vmArithmeticTest"
+
+to translate all the arithmetic tests.
+
+or, to translate a single test, run e.g.
+
+"ruby ./translate_test.rb ./Tests/vmArithmeticTest/add0Filler.json"
